update solutions

00-LeanInduction.lean
@@ -30,8 +30,18 @@ def sum_list (l : List Nat) : Nat :=
 
 /- HINT:  You may need a helper lemma -/
 
+theorem sum_list_helper: ∀ (l1 l2: List Nat), sum_list (l1 ++ l2) = sum_list l1 + sum_list l2 := by
+  intros l1 l2
+  induction l1
+  . case nil => simp [sum_list]
+  . case cons x xs ih => simp +arith [sum_list, ih]
+
 theorem sum_tree_contents : ∀ (t: Tree Nat), sum_tree t = sum_list (contents t) := by
- sorry
+  intros t
+  induction t
+  . case leaf => rfl
+  . case node l x r ih_r ih_l => simp +arith [sum_tree, contents, sum_list_helper, sum_list,
+    *]
 
 /- ***********************************************************************************
    Problem 2 (NK: exercise 2.7)
@@ -53,8 +63,10 @@ def post_order {α : Type} (t: Tree α) : List α :=
   | node l x r => post_order l ++ post_order r ++ [x]
 
 theorem mirror_order : ∀ {α : Type} (t: Tree α), pre_order (mirror t) = reverse (post_order t) := by
- sorry
-
+  intros α t
+  induction t
+  . case leaf => rfl
+  . case node l x r ih_l ih_r => simp +arith [mirror, pre_order, post_order, *]
 
 /- ***********************************************************************************
    Problem 3 (NK: exercise 2.8)
@@ -62,32 +74,54 @@ theorem mirror_order : ∀ {α : Type} (t: Tree α), pre_order (mirror t) = reve
 
 -- (a) First, complete the implementation of `intersp` so that `test_intersp` is automatically verified.
 def intersp {α : Type} (y: α) (xs : List α) : List α :=
- sorry
+  match xs with
+  | [] => []
+  | x :: [] => [x]
+  | x :: xs' => x :: y :: intersp y xs'
 
 theorem test_intersp : intersp 0 [1,2,3,4,5] = [1,0,2,0,3,0,4,0,5] := by rfl
 
 -- (b) Next, write a function `mymap` such that `test_map` is automatically verified
 def mymap {α β : Type} (f : α -> β) (xs: List α) : List β :=
- sorry
+  match xs with
+  | [] => []
+  | x :: xs' => f x :: mymap f xs'
 
 theorem test_mymap : mymap (λ x => x * 10) [1,2,3] = [10,20,30] := by rfl
 
 -- (c) Finally, prove the following theorem about `intersp` and `mymap`
 
 theorem map_intersperse : (∀ {α β : Type} (f: α -> β) (y: α) (xs: List α), map f (intersp y xs) = intersp (f y) (map f xs)) := by
- sorry
-
+  intros α β f y xs
+  induction xs with
+  | nil => rfl
+  | cons x xs ih =>
+    cases xs with
+    | nil => rfl
+    | cons x' xs' => simp [intersp, map, ih]
 
 /- ***********************************************************************************
    Problem 4 (NK: exercise 2.8)
    *********************************************************************************** -/
+
+open Nat
+
 def tail_rec_add (n m: Nat) : Nat :=
   match n with
-  | 0 => m
-  | n' + 1 => tail_rec_add n' (m + 1)
+  | zero => m
+  | succ n' => tail_rec_add n' (succ m)
+
+theorem tr_add_succ : ∀ (n m: Nat), tail_rec_add n (succ m) = succ (tail_rec_add n m) := by
+  intros n m
+  induction n generalizing m with
+  | zero => simp [tail_rec_add]
+  | succ n' ih => simp +arith [tail_rec_add, ih]
 
 theorem tail_rec_add_eq : ∀ (n m: Nat), tail_rec_add n m = n + m := by
- sorry
+  intros n m
+  induction n with
+  | zero => simp [tail_rec_add]
+  | succ n' ih => simp +arith [tail_rec_add, tr_add_succ, ih]
 
 /- ***********************************************************************************
    Problem 5 (NK: exercise 2.10)
@@ -126,7 +160,11 @@ def poly2 : Exp := Add poly1 poly0
 -- when you are done, `eval_test` should be automatically checked.
 
 def eval (e: Exp) (x: Nat) : Nat :=
- sorry
+  match e with
+  | Var => x
+  | Con n => n
+  | Exp.Add e1 e2 => eval e1 x + eval e2 x
+  | Exp.Mul e1 e2 => eval e1 x * eval e2 x
 
 theorem eval_test : eval poly2 5 = 65 := rfl
 
@@ -138,24 +176,69 @@ abbrev Poly := List Nat
 
 -- (b) Complete the implementation of `evalp` so that `evalp_test` succeeds automatically
 def evalp (p: Poly) (x: Nat) : Nat :=
- sorry
+  match p with
+  | [] => 0
+  | c :: p' => c + x * evalp p' x
 
 theorem evalp_test : evalp [10, 1, 2] 5 = eval poly2 5 := rfl
 
 -- (c) Complete the implementation of `coeffs` so that `coeffs_test` succeeds automatically
 -- HINT: you may need helper functions `addp` and `mulp` which *add* and *multiply* two `Poly`s
 
+def addp : Poly -> Poly -> Poly
+  | [], p => p
+  | p, [] => p
+  | c1 :: p1, c2 :: p2 => (c1 + c2) :: addp p1 p2
+
+def mulvp (v : Nat) (p : Poly) :=
+  mymap (λ x => v * x) p
+
+def mulp (p1 p2: Poly) : Poly :=
+  match p1, p2 with
+  | [], _ => []
+  | _, [] => []
+  | c1 :: p1', c2 :: p2' => c1 * c2 :: addp (mulvp c1 p2') (mulp p1' p2)
 
 def coeffs (e: Exp) : Poly :=
- sorry
+  match e with
+  | Var => [0, 1]
+  | Con n => [n]
+  | Exp.Add e1 e2 => addp (coeffs e1) (coeffs e2)
+  | Exp.Mul e1 e2 => mulp (coeffs e1) (coeffs e2)
 
 theorem coeffs_test : coeffs poly2 = [10, 1, 2] := by rfl
-
 
 -- (d) Complete the proof of `eval_poly`; HINT: you will likely
 -- require helper lemmas e.g. about the helper functions `addp` and `mulp`...
 
+theorem addp_helper : ∀ (p1 p2: Poly) (x: Nat), evalp (addp p1 p2) x = evalp p1 x + evalp p2 x := by
+  intros p1 p2 x
+  induction p1, p2 using addp.induct
+  . case case1 => simp [addp, evalp]
+  . case case2 => simp [addp, evalp]
+  . case case3 ih => simp +arith [addp, evalp, Nat.mul_add, ih]
 
+theorem mulvp_helper : ∀ (v: Nat) (p: Poly) (x: Nat), evalp (mulvp v p) x = v * evalp p x := by
+  intros v p x
+  induction p with
+  | nil => simp [mulvp, evalp, mymap]
+  | cons c cs ih => simp_all [mulvp, evalp, mymap, Nat.mul_add, mul_shuffle]
+
+theorem mulp_helper : ∀ (p1 p2: Poly) (x: Nat), evalp (mulp p1 p2) x = evalp p1 x * evalp p2 x := by
+  intros p1 p2 x
+  induction p1 with
+  | nil =>
+      simp [mulp, evalp]
+  | cons c1 p1' ih =>
+      cases p2 with
+      | nil => simp [mulp, evalp]
+      | cons c2 p2' =>
+          simp_all (arith := true) [mulp, evalp, addp_helper, mulvp_helper, Nat.mul_add, mul_shuffle, Nat.mul_comm]
 
 theorem eval_poly : ∀ (e:Exp) (x:Nat), evalp (coeffs e) x = eval e x := by
- sorry
+  intros e x
+  induction e with
+  | Var => simp [coeffs, evalp, eval]
+  | Con n => simp [coeffs, evalp, eval]
+  | Add e1 e2 ih1 ih2 => simp [coeffs, addp_helper, eval, ih1, ih2]
+  | Mul e1 e2 ih1 ih2 => simp [coeffs, mulp_helper, eval, ih1, ih2]
