01-Expressions.lean
@@ -58,8 +58,18 @@ def asimp_const (e: AExp) : AExp :=
 
 -- Complete the proof of lem_is_opt which states that `is_opt (asimp_const a)`
 --@[autogradedProof 20]
+
+/-
+x✝ : ∀ (n1 n2 : Val), asimp_const a✝¹ = AExp.num n1 → ¬asimp_const a✝ = AExp.num n2
+-/
+
 theorem optimal_asimp_const : ∀ {a: AExp}, is_opt (asimp_const a) = true := by
- sorry
+  intros a
+  induction a with
+  | num n => simp [asimp_const, is_opt]
+  | var x => simp [asimp_const, is_opt]
+  | plus e1 e2 ih1 ih2 =>
+    simp [asimp_const] <;> split <;> simp_all [is_opt]
 
 /- -------------------------------------------------------------------------------
    Q2: Next we will do a more serious transformation where expressions like
@@ -87,15 +97,22 @@ def unopt (a: AExpOpt) : AExp :=
 
 -- (a) Write a function that adds a constant to an optimized expression.
 def aoplusn (n : Val) (a: AExpOpt) : AExpOpt :=
- sorry
+  match a with
+  | AExpOpt.num n' => AExpOpt.num (n + n')
+  | AExpOpt.plus x a' => AExpOpt.plus x (aoplusn n a')
 
 -- (b) Next, write a function `aoplus` that adds two optimized expressions
 def aoplus (a other: AExpOpt) : AExpOpt :=
- sorry
+  match a with
+  | AExpOpt.num n1 => aoplusn n1 other
+  | AExpOpt.plus x a' => AExpOpt.plus x (aoplus a' other)
 
 -- (c) Write a function `asimp_opt` that converts plain expressions to optimized expressions.
 def asimp_opt (a: AExp) : AExpOpt :=
- sorry
+  match a with
+  | AExp.num n => AExpOpt.num n
+  | AExp.var x => AExpOpt.plus x (AExpOpt.num 0)
+  | AExp.plus e1 e2 => aoplus (asimp_opt e1) (asimp_opt e2)
 
 theorem add_silly : ∀ {x y z : Val}, x + (y + z) = y + (x + z) := by
   intros x y z
@@ -113,16 +130,40 @@ theorem add_silly : ∀ {x y z : Val}, x + (y + z) = y + (x + z) := by
 
  -/
 
+theorem aoplusn_helper : ∀ {n : Val} {a : AExpOpt} {s: State},
+  aval_opt (aoplusn n a) s = n + aval_opt a s := by
+  intros n a s
+  induction a with
+  | num n' => simp [aoplusn, aval_opt]
+  | plus x a' ih => simp [aoplusn, aval_opt, ih, add_silly]
+
+theorem aoplus_helper : ∀ {a1 a2 : AExpOpt} {s: State},
+  aval_opt (aoplus a1 a2) s = aval_opt a1 s + aval_opt a2 s := by
+  intros a1 a2 s
+  induction a1 with
+  | num n1 => simp [aoplus, aval_opt, aoplusn_helper]
+  | plus x a' ih => simp [aval_opt, aoplus, ih, Nat.add_assoc]
+
+  -- simp +arith [aoplus, aval_opt, ih, Nat.add_assoc]
 
 -- @[autogradedProof 30]
 theorem asimp_opt_aval : ∀ {a : AExp} {s: State},
   aval_opt (asimp_opt a) s = aval a s := by
- sorry
+  intros a s
+  induction a with
+  | num n => simp [asimp_opt, aval_opt, aval]
+  | var x => simp [asimp_opt, aval_opt, aval]
+  | plus e1 e2 ih1 ih2 =>
+    simp [asimp_opt, aval, aoplus_helper, ih1, ih2]
+
 
 -- @[autogradedProof 10]
 theorem unopt_aval : ∀ {a : AExpOpt} {s: State},
   aval (unopt a) s = aval_opt a s := by
- sorry
+  intros a s
+  induction a generalizing s with
+  | num n => simp [unopt, aval_opt, aval]
+  | plus x a' ih => simp [unopt, aval_opt, aval, ih]
 
 -- We can now define the "full simplification" function as
 def asimp_full (a : AExp) : AExp := unopt (asimp_opt a)
@@ -134,7 +175,9 @@ def asimp_full (a : AExp) : AExp := unopt (asimp_opt a)
 -- @[autogradedProof 10]
 theorem asimp_full_aval : ∀ {a : AExp} {s: State},
   aval (asimp_full a) s = aval a s := by
- sorry
+  intros a s
+  simp [asimp_full, unopt_aval, asimp_opt_aval]
+
 
 /- -------------------------------------------------------------------------------
    Q3:  Substitution `subst x a e` replaces all occurrences of variable `x` by
@@ -157,9 +200,14 @@ def subst (x: Vname) (a e: AExp) : AExp :=
 def asgn (x: Vname) (a: AExp) (s: State) : State := upd s x (aval a s)
 
 -- @[autogradedProof 20]
-theorem subst_lemma : ∀ { x: Vname } {a e: AExp} {s: State},
+theorem subst_lemma : ∀ {x: Vname} {a e: AExp} {s: State},
   aval (subst x a e) s = aval e (asgn x a s) := by
- sorry
+  intros x a e s
+  induction e generalizing s with
+  | var y => simp [subst] <;> split <;> simp_all [asgn, aval, upd]
+  | num n => simp [subst, aval]
+  | plus e1 e2 ih1 ih2 => simp_all [subst, aval]
+
 
 -- HINT: when you get to the `if` you may want to use the `split` tactic as illustrated below.
 
@@ -197,7 +245,7 @@ def lval (e: LExp) (s: State) : Val :=
   | LExp.num n => n
   | LExp.var x => s x
   | LExp.plus e1 e2 => lval e1 s + lval e2 s
-  | LExp.llet x e1 e2 => lval e2 (upd s x (lval e1 s))
+  | LExp.llet x e1 e2 => lval e2 (upd s x (lval e1 s)) -- let x = e1 in e2
 
 -- Write a function `inlyne` that converts an `LExp` into a plain `AExp`
 -- by "inlining" the let-definitions, i.e. `let x = e1 in e2` should become
@@ -205,12 +253,21 @@ def lval (e: LExp) (s: State) : Val :=
 
 -- @[autogradedProof 15]
 def inlyne (e: LExp) : AExp :=
- sorry
+  match e with
+  | LExp.num n => AExp.num n
+  | LExp.var x => AExp.var x
+  | LExp.plus e1 e2 => AExp.plus (inlyne e1) (inlyne e2)
+  | LExp.llet x e1 e2 => subst x (inlyne e1) (inlyne e2)
 
 -- Prove that your `inlyne` function is correct; HINT: recall the `subst_lemma`
 -- @[autogradedProof 30]
 theorem inlyne_sound: ∀ {e : LExp} {s: State}, lval e s = aval (inlyne e) s := by
- sorry
+  intros e s
+  induction e generalizing s with
+  | num n => simp [inlyne, lval, aval]
+  | var x => simp [inlyne, lval, aval]
+  | plus e1 e2 ih1 ih2 => simp [inlyne, lval, aval, ih1, ih2]
+  | llet x e1 e2 ih1 ih2 => simp_all [inlyne, lval, subst_lemma, asgn]
 
 /- -----------------------------------------------------------------------------
    Q5: Palindromes
@@ -223,7 +280,11 @@ inductive palindrome : List Nat -> Prop where
 
 -- @[autogradedProof 10]
 theorem palindrome_rev : ∀ (ns : List Nat), (palindrome ns) -> List.reverse ns = ns := by
- sorry
+  intros ns pal
+  induction pal with
+  | emp => rfl
+  | sng n => rfl
+  | cns n ns' pal' ih => simp_all []
 
 /- -----------------------------------------------------------------------------
    Q6: Even numbers revisited
@@ -235,7 +296,7 @@ inductive Ev : Nat -> Prop where
   | evss :  ∀ {n : Nat}, Ev n -> Ev ((n + 1) + 1)
 
 theorem another_add_silly : ∀ {k : Nat}, k + 1 + (k + 1) = ((k + k) + 1 ) + 1 := by
-  intros k; simp_arith []
+  intros k; simp +arith []
 
 theorem double_ev : ∀ {n : Nat}, (∃ k, n = k + k) -> Ev n := by
   intros n double
@@ -249,7 +310,11 @@ theorem double_ev : ∀ {n : Nat}, (∃ k, n = k + k) -> Ev n := by
 
 -- @[autogradedProof 15]
 theorem ev_double : ∀ {n : Nat}, Ev n -> ∃ k, n = k + k := by
- sorry
+  intros n ev
+  induction ev with
+  | evz => exists 0
+  | evss ev' ih =>
+    cases ih with | intro k n_eq_2k => exists (k + 1); simp_all [another_add_silly]
 
 /- -----------------------------------------------------------------------------
    Q7: Iteration
@@ -270,6 +335,13 @@ inductive iter {α : Type} (r : α -> α -> Prop) : Nat -> α -> α -> Prop wher
 
 -- @[autogradedProof 15]
 theorem star_iter : ∀ {α : Type} {r : α -> α -> Prop} {a b : α},
-  star r a b -> ∃ (n : Nat), iter r n a b :=
-  by
- sorry
+  star r a b -> ∃ (n : Nat), iter r n a b := by
+  intros α r a b star_ab
+  induction star_ab with
+  | refl => exists 0; apply iter.iter_base
+  | step r' _ ih =>
+    cases ih with | intro n iter_r'_n_a_b =>
+      exists (n + 1)
+      apply iter.iter_step
+      assumption
+      assumption
