05-STLC.lean
@@ -35,15 +35,15 @@ inductive Op where
 open Op
 
 inductive Exp where
-  | ENum : Int -> Exp
-  | EBool: Bool -> Exp
-  | EVar : Vname -> Exp
-  | EOp  : Op -> Exp -> Exp -> Exp
-  | ELam : Vname -> Ty -> Exp -> Exp
-  | EApp : Exp -> Exp -> Exp
-  | EIf  : Exp -> Exp -> Exp -> Exp
--- **EC**
+  | ENum : Int -> Exp                     -- 0, 1, 2, 3 ...
+  | EBool: Bool -> Exp                    -- true, false
+  | EVar : Vname -> Exp                   -- x, y, z ...
+  | EOp  : Op -> Exp -> Exp -> Exp        -- e1 ⊗ e2
+  | ELam : Vname -> Ty -> Exp -> Exp      -- λ x : τ => e
+  | EApp : Exp -> Exp -> Exp              -- e1 e2
+  | EIf  : Exp -> Exp -> Exp -> Exp       -- if b then e1 else e2
   | ERec : Vname -> Vname -> Ty -> Ty -> Exp -> Exp
+                                          -- rec succ (x : int) : int = (if x = 0 then 0 else x + 1)
   deriving Repr
 open Exp
 
@@ -104,8 +104,7 @@ inductive Val where
   | VInt   : Int -> Val
   | VBool  : Bool -> Val
   | VClos  : Vname -> Ty -> Exp -> (Vname -> Val) -> Val
-  -- **EC** You may need to add cases for `ERec`
-
+  | VRec   : Vname -> Vname -> Ty -> Ty -> Exp -> (Vname -> Val) -> Val
 open Val
 
 /- @@@
@@ -162,13 +161,18 @@ def eval (k : Nat) (ρ : Store) (e : Exp) : Result Val :=
     | EVar x      => Ok (ρ x)
     | EOp o e1 e2 => combine (eval k ρ e1) (eval k ρ e2) (eval_op o)
     | ELam x τ e  => Ok (VClos x τ e ρ)
-    | EApp e1 e2  => combine  (eval k ρ e1) (eval k ρ e2) (fun v1 v2 =>
+    | EApp e1 e2  => combine (eval k ρ e1) (eval k ρ e2) (fun v1 v2 =>
                        match v1 with
                        | VClos x _ e ρ' => eval k (ρ' [ x := v2 ]) e
+                       | VRec f x _ _ e ρ' => eval k (ρ' [ x := v2 ][ f := v1 ]) e
                        | _ => Stuck
                      )
-    | EIf b e1 e2 => sorry
-    | ERec f x t t' e => sorry
+    | EIf b e1 e2 => match eval k ρ b with
+                       | Ok (VBool true)  => eval k ρ e1
+                       | Ok (VBool false) => eval k ρ e2
+                       | Timeout => Timeout
+                       | _ => Stuck
+    | ERec f x τ τ' e => Ok (VRec f x τ τ' e ρ)
 
 /- @@@
 ### Tests!
@@ -236,6 +240,14 @@ inductive WT : Env -> Exp -> Ty -> Prop where
              WT Γ e1 (TFun τ τ') -> WT Γ e2 τ ->
              WT Γ (EApp e1 e2) τ'
 
+  | TIf    : ∀ {b e1 e2 τ},
+             WT Γ b TBool -> WT Γ e1 τ -> WT Γ e2 τ ->
+             WT Γ (EIf b e1 e2) τ
+
+  | TRec   : ∀ {f x τ τ' e},
+              WT (Γ [ x := τ ] [ f := TFun τ τ' ]) e τ' ->
+              WT Γ (ERec f x τ τ' e) (TFun τ τ')
+
 
 notation:10 Γ "⊢" e ":" t => WT Γ e t
 
@@ -251,6 +263,7 @@ theorem tyChoose : Γ₀ ⊢ eChoose : TFun TBool (TFun TInt (TFun TInt TInt))
 -- @[autogradedProof 10]
 theorem tySum : Γ₀ ⊢ eSum : TFun TInt TInt
   := by repeat constructor
+
 
 /- --------------------------------------------------------------------------------------------
 ## Type Soundness
@@ -273,6 +286,9 @@ inductive WV : Val -> Ty -> Prop where
 
   | TVClos  : (∀ x, WV (ρ x) (Γ x)) -> WT (Γ [ x := τ ]) e τ' ->
               WV (VClos x τ e ρ) (TFun τ τ')
+
+  | TVRec   : (∀ x, WV (ρ x) (Γ x)) -> WT (Γ [ x := τ ] [ f := TFun τ τ' ]) e τ' ->
+              WV (VRec f x τ τ' e ρ) (TFun τ τ')
 
   -- **EC** you may need to add cases for the extra `Val` cases defined above.
 
@@ -300,7 +316,7 @@ abbrev WS (Γ : Env) (ρ : Store) := ∀ x, (⊢ ρ x : Γ x)
 
 notation:10 Γ "⊢" ρ  => WS Γ ρ
 
-@[simp]
+-- @[simp]
 theorem int_val : ∀ {v: Val}, (⊢ v : TInt) <-> (∃ i, v = VInt i)
   := by
   intros v
@@ -308,7 +324,7 @@ theorem int_val : ∀ {v: Val}, (⊢ v : TInt) <-> (∃ i, v = VInt i)
   . case mp => intros wv; cases wv; rename_i i; apply Exists.intro; trivial
   . case mpr => intro h ; cases h ; simp_all []; constructor
 
-@[simp]
+-- @[simp]
 theorem bool_val : ∀ {v: Val}, (⊢ v : TBool) <-> (∃ b, v = VBool b)
   := by
   intros v
@@ -323,7 +339,26 @@ theorem op_safe: ∀ {v1 v2 : Val} {o τ1 τ2},
   (⊢ v1 : τ1) -> (⊢ v2 : τ2) -> some τ = ty_op o τ1 τ2 ->
   ∃ v, eval_op o v1 v2 = Ok v ∧ WV v τ
   := by
-  sorry
+  intros v1 v2 o τ1 τ2 wv1 wv2 h_ty_op
+  cases o
+  . case Add =>
+    have τi_t : τ1 = TInt ∧ τ2 = TInt := by
+      constructor <;> cases τ1 <;> cases τ2 <;> simp_all [ty_op]
+    have τ_t : τ = TInt := by
+      cases τi_t; simp_all [ty_op]
+    simp_all
+    cases wv1; cases wv2
+    simp_all [eval_op, op_add]
+    constructor
+  · case Equal =>
+    have τi_int : τ1 = TInt -> τ2 = TInt := by
+      intro τ1_int; cases τ2 <;> simp_all [ty_op]
+    have τi_bool : τ1 = TBool -> τ2 = TBool := by
+      intro τ1_bool; cases τ2 <;> simp_all [ty_op]
+    cases τ1 <;> cases τ2 <;> simp_all [ty_op] <;>
+    cases wv1 <;> cases wv2 <;>
+    simp_all [eval_op, op_equal] <;>
+    constructor
 
 
 -- **Problem 4** Complete the proof of `op_safe` ------------------------------------
@@ -333,7 +368,15 @@ theorem op_safe_r : ∀ {r1 r2 : Result Val} {τ1 τ2 o},
   (⊢ r1 : τ1) -> (⊢ r2 : τ2) -> some τ = ty_op o τ1 τ2 ->
   (⊢ combine r1 r2 (eval_op o) : τ)
   := by
-  sorry
+  intros r1 r2 τ1 τ2 o wr1 wr2 h_ty_op
+  cases r1 <;> cases r2 <;> cases wr1 <;> cases wr2 <;> simp_all [combine]
+  . case Ok.Ok v1 v2 _ _ =>
+    obtain ⟨ v, eval_op_v ⟩ : ∃ v, eval_op o v1 v2 = Ok v ∧ (⊢ v : τ) := by apply op_safe <;> assumption
+    cases eval_op_v
+    simp_all
+    constructor
+    assumption
+  repeat constructor
 
 -- lemma 2
 theorem lookup_safe : ∀ {Γ ρ x},
@@ -363,7 +406,86 @@ theorem wr_val : ∀ { r τ },
 theorem eval_safe: ∀ {Γ e τ ρ k },
   (Γ ⊢ e : τ) -> (Γ ⊢ ρ) -> (⊢ eval k ρ e : τ)
   := by
-  sorry
+  intros Γ e τ ρ k h_wt h_ws
+  induction k, ρ, e using eval.induct generalizing Γ τ
+  . case case1 => simp_all [eval]; constructor  -- k = 0
+  . case case2 => cases h_wt; simp_all [eval]; repeat constructor  -- num
+  . case case3 => cases h_wt; simp_all [eval]; repeat constructor  -- bool
+  . case case4 => cases h_wt; simp_all [eval]; constructor; simp_all  -- var
+  . case case5 ih1 ih2 =>  -- op
+    cases h_wt
+    simp_all [eval]; apply op_safe_r
+    apply ih1; repeat assumption
+    apply ih2; repeat assumption
+    simp_all []
+  . case case6 =>  -- lam
+    cases h_wt
+    simp_all [eval]
+    repeat constructor
+    repeat assumption
+  . case case7 ρ k e1 e2 ih1 ih2 ih3 ih4 =>  -- app
+    cases k
+    . case zero => simp_all [eval, combine]; constructor
+    . case succ k' =>
+      cases h_wt
+      rename_i τ' wt2 wt1
+      have eval_v1 : ¬ (eval (k' + 1) ρ e1 = Timeout) -> ∃ v1, eval (k' + 1) ρ e1 = Ok v1 ∧ (⊢ v1 : TFun τ' τ) := by
+        intros; apply wr_val; assumption; apply ih1; repeat assumption
+      have eval_v2 : ¬ (eval (k' + 1) ρ e2 = Timeout) -> ∃ v2, eval (k' + 1) ρ e2 = Ok v2 ∧ (⊢ v2 : τ') := by
+        intros; apply wr_val; assumption; apply ih2; repeat assumption
+      cases r1 : eval (k' + 1) ρ e1 <;> cases r2 : eval (k' + 1) ρ e2 <;> simp_all
+      . case TApp.Ok.Ok v1 v2 =>
+        cases eval_v1 <;> simp_all [eval.eq_7, combine]
+        . case TVClos =>
+          apply ih3
+          assumption
+          apply ws_upd
+          repeat assumption
+        . case TVRec =>
+          apply ih4
+          assumption
+          apply ws_upd
+          apply ws_upd
+          assumption
+          assumption
+          constructor
+          assumption
+          assumption
+      . case TApp.Ok.Timeout =>
+        cases eval_v1 <;> simp_all [eval.eq_7, combine] <;> constructor
+      . case TApp.Timeout.Ok =>
+        simp_all [eval.eq_7, combine]
+        constructor
+      . case TApp.Timeout.Timeout =>
+        simp_all [eval.eq_7, combine]
+        constructor
+  . case case8 ih =>  -- if true
+    cases h_wt
+    simp_all [eval]
+    apply ih
+    repeat assumption
+  . case case9 ih => -- if false
+    cases h_wt
+    simp_all [eval]
+    apply ih
+    assumption
+    assumption
+  . case case10 => simp_all [eval]; constructor
+  . case case11 ρ k b e1 e2 b_true b_false not_timeout ih =>
+    cases h_wt
+    rename_i wtb wt1 wt2
+    obtain ⟨ bv, eval_b ⟩ : ∃ bv, eval k ρ b = Ok bv ∧ (⊢ bv : TBool) := by
+      intros; apply wr_val; assumption; apply ih; repeat assumption
+    cases eval_b
+    rename_i eval_b bv_t
+    rw [bool_val] at bv_t
+    simp_all
+  . case case12 ρ k f x τ' τ'' e =>
+    cases h_wt
+    simp_all [eval]
+    repeat constructor
+    repeat assumption
+
 
 /- @@@ --------------------------------------------------------------------------------------------
 ## A Type Checker
@@ -382,7 +504,7 @@ theorem eval_safe: ∀ {Γ e τ ρ k },
   intros t1 t2; constructor
   . case mp =>
     intros eqTy
-    induction t1 generalizing t2 <;> cases t2 <;> simp_all [eqTy]
+    induction t1 generalizing t2 <;> cases t2 <;> simp_all []
     rename_i t1 t1' ih1 ih2 t2 t2'
     cases eqTy
     constructor
@@ -398,7 +520,38 @@ theorem eval_safe: ∀ {Γ e τ ρ k },
 -- `checkInc`, `checkChoose` (and for EC `checkSum`) automatically verify.
 
 @[simp] def check (Γ : Env) (e : Exp) : Option Ty :=
-  sorry
+  match e with
+  | ENum _      => some TInt
+  | EBool _     => some TBool
+  | EVar x      => some (Γ x)
+  | EOp o e1 e2 => do
+      match check Γ e1 with
+      | some τ1 =>
+        match check Γ e2 with
+        | some τ2 => ty_op o τ1 τ2
+        | _ => none
+      | _ => none
+  | ELam x τ e  =>
+      match check (Γ [ x := τ ]) e with
+      | some τ' => some (TFun τ τ')
+      | none => none
+  | EApp e1 e2  =>
+      match check Γ e1, check Γ e2 with
+      | some (TFun τ' τ''), some τ =>
+          if eqTy τ' τ then some τ'' else none
+      | _, _ => none
+  | EIf b e1 e2 =>
+      match check Γ b with
+      | some TBool =>
+        match check Γ e1, check Γ e2 with
+        | some τ1, some τ2 =>
+            if eqTy τ1 τ2 then some τ1 else none
+        | _, _ => none
+      | _ => none
+  | ERec f x τ τ' e =>
+      match check (Γ [ x := τ ] [ f := TFun τ τ' ]) e with
+      | some τ'' => if eqTy τ' τ'' then some (TFun τ τ') else none
+      | _ => none
 
 
 -- @[autogradedProof 10]
@@ -417,7 +570,11 @@ theorem checkSum : check Γ₀ eSum = some (TFun TInt TInt) := rfl
 theorem checkOp_sound: ∀ { Γ o e1 e2 t1 t2 t},
   (Γ ⊢ e1 : t1) -> (Γ ⊢ e2 : t2) -> some t = ty_op o t1 t2 -> (Γ ⊢ EOp o e1 e2 : t)
   := by
-  sorry
+  intros Γ o e1 e2 t1 t2 t h_wt1 h_wt2 h_ty_op
+  constructor
+  assumption
+  assumption
+  simp_all
 
 -- **Problem 7** Complete the proof of `check_sound`
 
@@ -425,4 +582,23 @@ theorem checkOp_sound: ∀ { Γ o e1 e2 t1 t2 t},
 theorem check_sound : ∀ { Γ e t },
   some t = check Γ e -> ( Γ ⊢ e : t )
   := by
-  sorry
+  intros Γ e t h_check
+  induction Γ, e using check.induct generalizing t
+  . case case1 => simp_all; constructor
+  . case case2 => simp_all; constructor
+  . case case3 => simp_all; constructor
+  . case case4 ih1 ih2 => simp_all; constructor; assumption; assumption; simp_all
+  . case case5 => simp_all
+  . case case6 => simp_all
+  . case case7 ih => simp_all; constructor; assumption
+  . case case8 => simp_all
+  . case case9 ih1 ih2 => simp_all; constructor; repeat assumption
+  . case case10 => simp_all
+  . case case11 => simp_all
+  . case case12 => simp_all; constructor; repeat assumption
+  . case case13 => simp_all
+  . case case14 => simp_all
+  . case case15 => simp_all
+  . case case16 r_check _ ih =>  rw [r_check] at ih; simp_all; constructor; assumption
+  . case case17 => simp_all
+  . case case18 => simp_all
